Auto/Embedding/LamInference.lean
@@ -2,44 +2,42 @@ import Auto.Embedding.LamConv
 
 namespace Auto.Embedding.Lam
 
-def LamTerm.elimBVar? (t : LamTerm) : Option LamTerm :=
-  match t.hasLooseBVarEq 0 with
-  | false => .some (LamTerm.instantiate1 (.atom 0) t)
-  | true => .none
+theorem LamValid.bvarLowers?
+  (hv : LamValid lval (pushLCtxs ss lctx) t)
+  (hlvl : ss.length = lvl)
+  (heq : LamTerm.bvarLowers? lvl t = .some t')
+  (hInh : HList (LamNonempty lval.tyVal) ss) :
+  LamValid lval lctx t' := by
+  cases LamTerm.bvarLowers?_spec.mp heq
+  have ⟨wft', ht'⟩ := hv; have hInh' := hInh.map (fun s inh => Classical.choice inh)
+  exists LamWF.fromBVarLifts hlvl _ wft'; intro lctxTerm
+  have ht'' := ht' (pushLCtxsDep hInh' lctxTerm)
+  rw [LamWF.interp_ofBVarLifts lval hInh' hlvl]; apply Eq.mp _ ht''
+  apply congrArg; apply LamWF.interp_substWF
 
-theorem LamTerm.maxEVarSucc_elimBVarIdx?
-  (heq : LamTerm.elimBVar? t = .some t') : t'.maxEVarSucc = t.maxEVarSucc := by
-  dsimp [LamTerm.elimBVar?] at heq; cases h : hasLooseBVarEq 0 t <;> rw [h] at heq <;> cases heq
-  rw [maxEVarSucc_instantiate1, h]
+theorem LamThmValid.bvarLowers?
+  (hv : LamThmValid lval (ss ++ lctx) t)
+  (hlvl : ss.length = lvl)
+  (heq : LamTerm.bvarLowers? lvl t = .some t')
+  (hInh : HList (LamNonempty lval.tyVal) ss) :
+  LamThmValid lval lctx t' := fun lctx' =>
+  have hv' := hv lctx'; LamValid.bvarLowers? (by rw [pushLCtxs_append] at hv'; exact hv') hlvl heq hInh
 
-theorem LamThmValid.elimBVarIdx? (hv : LamThmValid lval (s :: lctx) t)
-  (heq : LamTerm.elimBVar? t = .some t') (hInh : LamNonempty lval.tyVal s) :
-  LamThmValid lval lctx t' := by
-  dsimp [LamTerm.elimBVar?] at heq; cases h : t.hasLooseBVarEq 0 <;> rw [h] at heq <;> cases heq
-  have sinh := hInh.get
-  let lval' :=
-    {lval with lamEVarTy := fun n => match n.blt t.maxEVarSucc with | true => lval.lamEVarTy n | false => s
-               eVarVal := fun n => by simp [LamSort.interp]; match n.blt t.maxEVarSucc with | true => exact lval.eVarVal n | false => exact sinh}
-  have meeq : (LamTerm.instantiate1 (LamTerm.atom 0) t).maxEVarSucc = t.maxEVarSucc := by
-    rw [LamTerm.maxEVarSucc_instantiate1]; cases LamTerm.hasLooseBVarEq 0 t <;> dsimp
-    case true => simp [LamTerm.maxEVarSucc, Nat.max, Nat.max_zero_left]
-  have hirr : ∀ (n : Nat), n < t.maxEVarSucc →
-    lval'.lamEVarTy n = lval.lamEVarTy n ∧ HEq (lval'.eVarVal n) (lval.eVarVal n) := by
-    intro n; dsimp
-    match h : n.blt t.maxEVarSucc with
-    | true => dsimp; intro _; apply And.intro rfl HEq.rfl
-    | false =>
-      rw [← Bool.eq_false_eq_not_eq_true] at h;
-      dsimp at h; rw [Nat.blt_eq] at h; intro h'; apply False.elim (h h')
-  apply LamThmValid.eVarIrrelevance lval' lval rfl rfl HEq.rfl HEq.rfl HEq.rfl rfl (by rw [meeq]; exact hirr) ?valid
-  rw [LamTerm.instantiate1_bVarIrrelevance (arg₂ := (.etom t.maxEVarSucc)) h]
-  apply LamThmValid.instantiate1 (argTy:=s)
-  case hw =>
-    intro lctx'; apply LamWF.ofEtom'; dsimp [Nat.blt]
-    rw [(Nat.ble_eq_false_eq_lt _).mp .refl]
-  case hv =>
-    apply LamThmValid.eVarIrrelevance lval lval' rfl rfl HEq.rfl HEq.rfl HEq.rfl rfl _ hv
-    intro n h'; apply And.intro (hirr n h').left.symm (hirr n h').right.symm
+theorem LamValid.bvarLower?
+  (hv : LamValid lval (pushLCtx s lctx) t)
+  (heq : LamTerm.bvarLower? t = .some t')
+  (hInh : LamNonempty lval.tyVal s) :
+  LamValid lval lctx t' :=
+  LamValid.bvarLowers? (ss:=[s])
+    (by rw [pushLCtxs_singleton]; exact hv)
+    rfl heq (HList.cons hInh HList.nil)
+
+theorem LamThmValid.bvarLower?
+  (hv : LamThmValid lval (s :: lctx) t)
+  (heq : LamTerm.bvarLower? t = .some t')
+  (hInh : LamNonempty lval.tyVal s) :
+  LamThmValid lval lctx t' := fun lctx' =>
+  have hv' := hv lctx'; LamValid.bvarLower? (by rw [pushLCtxs_cons] at hv'; exact hv') heq hInh
 
 def LamTerm.impApp? (t₁₂ t₁ : LamTerm) : Option LamTerm :=
   match t₁₂ with
